pcuic/theories/PCUICSpine.v
@@ -1,0 +1,638 @@
+(* Distributed under the terms of the MIT license.   *)
+
+From Coq Require Import Bool String List Program BinPos Compare_dec Arith Lia
+     Classes.CRelationClasses ProofIrrelevance ssreflect.
+From MetaCoq.Template Require Import config Universes monad_utils utils BasicAst
+     AstUtils UnivSubst.
+From MetaCoq.PCUIC Require Import PCUICAst PCUICAstUtils PCUICInduction
+     PCUICReflect PCUICLiftSubst PCUICUnivSubst PCUICTyping PCUICUnivSubstitution
+     PCUICCumulativity PCUICPosition PCUICEquality PCUICNameless
+     PCUICAlpha PCUICNormal PCUICInversion PCUICCumulativity PCUICReduction
+     PCUICConfluence PCUICConversion PCUICContextConversion PCUICValidity
+     PCUICParallelReductionConfluence PCUICWeakeningEnv
+     PCUICClosed PCUICPrincipality PCUICSubstitution
+     PCUICWeakening PCUICGeneration PCUICUtils PCUICCtxShape PCUICContexts
+     PCUICUniverses PCUICArities.
+From Equations Require Import Equations.
+
+Require Import Equations.Prop.DepElim.
+Require Import Equations.Type.Relation_Properties.
+
+Derive Signature for typing_spine.
+  
+Notation ctx_inst Σ Γ i Δ := (ctx_inst (lift_typing typing) Σ Γ i Δ).
+
+Lemma typing_spine_strengthen {cf:checker_flags} Σ Γ T args U : 
+  wf Σ.1 ->
+  typing_spine Σ Γ T args U ->
+  forall T', Σ ;;; Γ |- T' <= T ->
+  typing_spine Σ Γ T' args U.
+Proof.
+  induction 2 in |- *; intros T' (*WAT*)redT.
+  - constructor. eauto. transitivity ty; auto.
+  - specialize (IHX0 (B {0 := hd})).
+    forward IHX0. { reflexivity. }
+    eapply type_spine_cons with na A B; auto.
+    etransitivity; eauto.
+Qed.
+
+Lemma subslet_app {cf:checker_flags} Σ Γ s s' Δ Δ' : 
+  subslet Σ Γ s (subst_context s' 0 Δ) ->
+  subslet Σ Γ s' Δ' ->
+  subslet Σ Γ (s ++ s') (Δ' ,,, Δ).
+Proof.
+induction Δ in s, s', Δ' |- *; simpl; auto; move=> sub'.
+- depelim sub'. auto.
+- rewrite subst_context_snoc in sub' => sub''.
+  move:(subslet_length sub') => /=.
+  rewrite /snoc /= subst_context_length /= => Hlen.
+  destruct a as [na [b|] ty].
+  * depelim sub'; simpl in H; noconf H.
+    simpl in t0, Hlen.
+    rewrite -subst_app_simpl' /=. lia.
+    constructor. eauto.
+    now rewrite - !subst_app_simpl' in t0; try lia.
+  * rewrite /subst_decl /map_decl /snoc /= in sub'.
+    depelim sub'; simpl in H; noconf H. simpl in Hlen.
+    rewrite - !subst_app_simpl' in t0; try lia.
+    simpl; constructor; eauto.
+Qed.
+
+Lemma context_subst_app_inv {ctx ctx' : list PCUICAst.context_decl} {args s : list term} :
+  context_subst (subst_context (skipn #|ctx| s) 0 ctx)
+    (skipn (PCUICAst.context_assumptions ctx') args) 
+    (firstn #|ctx| s)
+  × context_subst ctx' (firstn (PCUICAst.context_assumptions ctx') args)	(skipn #|ctx| s) ->
+  context_subst (ctx ++ ctx') args s.
+Proof.
+  move=> [Hl Hr].
+  rewrite -(firstn_skipn (context_assumptions ctx') args).
+  assert (lenctx' : context_assumptions ctx' + context_assumptions ctx = #|args|).
+  { assert (lenctx'' : context_assumptions ctx' <= #|args|).
+    move: (context_subst_assumptions_length _ _ _ Hr).
+    rewrite firstn_length; lia.
+    move: (context_subst_assumptions_length _ _ _ Hr).
+    move: (context_subst_assumptions_length _ _ _ Hl).
+    rewrite firstn_length skipn_length; try lia.
+    intros H1 H2. rewrite context_assumptions_subst in H1. lia. }
+  move: args s ctx' lenctx' Hl Hr.
+  induction ctx => args s ctx' lenctx' Hl Hr.
+  - simpl in *. depelim Hl. rewrite H app_nil_r. now rewrite skipn_0 in Hr.
+  - simpl in *. destruct s as [|u s];
+    simpl in *; rewrite subst_context_snoc0 in Hl; depelim Hl.
+    simpl in H. noconf H.
+    * destruct a as [na [b|] ty]; simpl in *; noconf H.
+      rewrite skipn_S in Hl, Hr. destruct args using rev_case. rewrite skipn_nil in H0.
+      apply (f_equal (@length _)) in H0. simpl in H0. autorewrite with len in H0.
+      simpl in H0; lia. rewrite H0.
+      rewrite skipn_app in H0.
+      rewrite app_length /= in lenctx'.
+      specialize (IHctx args s ctx'). forward IHctx by lia.
+      assert (context_assumptions ctx' - #|args| = 0) by lia.
+      rewrite H skipn_0 in H0. apply app_inj_tail in H0 as [Ha xu]. subst x.
+      rewrite -Ha.
+      rewrite -Ha in Hl. specialize (IHctx Hl).
+      rewrite firstn_app in Hr |- *.
+      rewrite H [firstn _ [u]]firstn_0 // app_nil_r in Hr |- *.
+      specialize (IHctx Hr). rewrite app_assoc.
+      now econstructor.
+    * destruct a as [na' [b'|] ty']; simpl in *; simpl in H; noconf H. simpl in H.
+      rewrite skipn_S in Hl, Hr, H. rewrite -H.
+      pose proof (context_subst_length _ _ _ Hl). rewrite subst_context_length in H0.
+      rewrite {3}H0 -subst_app_simpl [firstn #|ctx| _ ++ _]firstn_skipn. constructor.
+      apply IHctx => //.
+Qed.
+
+
+Lemma ctx_inst_inst {cf:checker_flags} Σ ext u Γ i Δ  :
+  wf_global_ext Σ.1 ext ->
+  ctx_inst (Σ.1, ext) Γ i Δ ->
+  consistent_instance_ext Σ ext u ->
+  ctx_inst Σ (subst_instance_context u Γ)
+    (map (subst_instance_constr u) i)
+    (subst_instance_context u Δ).
+Proof.
+  intros wfext ctxi cu.
+  induction ctxi; simpl; constructor; auto.
+  * red in p |- *.
+    destruct Σ as [Σ univs].
+    eapply (typing_subst_instance'' Σ); eauto. apply wfext.
+    apply wfext.
+  * rewrite (subst_telescope_subst_instance_constr u [i]).
+    apply IHctxi.
+  * rewrite (subst_telescope_subst_instance_constr u [b]).
+    apply IHctxi.
+Qed.
+
+Lemma subst_type_local_ctx {cf:checker_flags} Σ Γ Γ' Δ Δ' s ctxs : 
+  wf Σ.1 ->
+  wf_local Σ (Γ ,,, Δ ,,, Γ') ->
+  type_local_ctx (lift_typing typing) Σ (Γ ,,, Δ ,,, Γ') Δ' ctxs ->
+  subslet Σ Γ s Δ ->
+  type_local_ctx (lift_typing typing) Σ (Γ ,,, subst_context s 0 Γ') (subst_context s #|Γ'| Δ') ctxs.
+Proof.
+  induction Δ' in Γ' |- *; simpl; auto.
+  destruct a as [na [b|] ty]; simpl; intuition auto.
+  + destruct a0; simpl; rewrite subst_context_snoc /= /subst_decl /map_decl /=.
+    intuition auto.
+    - exists x; auto.
+      rewrite -app_context_assoc in t.
+      eapply substitution in t; eauto.
+      rewrite subst_context_app app_context_assoc in t.
+      simpl in t. rewrite Nat.add_0_r in t. 
+      now rewrite app_context_length in t.
+    - rewrite -app_context_assoc in b1.
+      eapply substitution in b1; eauto.
+      rewrite subst_context_app app_context_assoc Nat.add_0_r in b1.
+      now rewrite app_context_length in b1.
+  + rewrite subst_context_snoc /= /subst_decl /map_decl /=.
+      intuition auto.
+      rewrite -app_context_assoc in b.
+      eapply substitution in b; eauto.
+      rewrite subst_context_app app_context_assoc in b.
+      rewrite Nat.add_0_r in b. 
+      now rewrite app_context_length in b.
+Qed.
+
+Record spine_subst {cf:checker_flags} Σ Γ inst s Δ := mkSpineSubst {
+  spine_dom_wf : wf_local Σ Γ;
+  spine_codom_wf : wf_local Σ (Γ ,,, Δ);
+  inst_ctx_subst :> context_subst Δ inst s;
+  inst_subslet :> subslet Σ Γ s Δ }.
+Arguments inst_ctx_subst {cf Σ Γ inst s Δ}.
+Arguments inst_subslet {cf Σ Γ inst s Δ}.
+Hint Resolve inst_ctx_subst inst_subslet : pcuic.
+
+Lemma spine_subst_eq {cf:checker_flags} {Σ Γ inst s Δ Δ'} : 
+  spine_subst Σ Γ inst s Δ ->
+  Δ = Δ' ->
+  spine_subst Σ Γ inst s Δ'.
+Proof.
+  now intros sp ->.
+Qed.
+
+Inductive arity_spine {cf : checker_flags} (Σ : PCUICAst.global_env_ext) (Γ : PCUICAst.context) : 
+  term -> list term -> term -> Type :=
+| arity_spine_nil ty ty' :
+  isWfArity_or_Type Σ Γ ty' ->
+  Σ ;;; Γ |- ty <= ty' ->
+  arity_spine Σ Γ ty [] ty'
+| arity_spine_def : forall (tl : list term) 
+                      (na : name) (A a B B' : term),                      
+                    arity_spine Σ Γ (B {0 := a}) tl B' ->
+                    arity_spine Σ Γ (tLetIn na a A B) tl B'
+| arity_spine_ass : forall (hd : term) (tl : list term) 
+                      (na : name) (A B B' : term),
+                    Σ;;; Γ |- hd : A ->
+                    arity_spine Σ Γ (B {0 := hd}) tl B' ->
+                    arity_spine Σ Γ (tProd na A B) (hd :: tl) B'.
+
+Record wf_arity_spine {cf:checker_flags} Σ Γ T args T' :=
+{ wf_arity_spine_wf : isWfArity_or_Type Σ Γ T;
+  wf_arity_spine_spine : arity_spine Σ Γ T args T' }.
+
+Lemma wf_arity_spine_typing_spine {cf:checker_flags} Σ Γ T args T' :
+  wf Σ.1 ->
+  wf_arity_spine Σ Γ T args T' ->
+  typing_spine Σ Γ T args T'.
+Proof.
+  intros wfΣ [wf sp].
+  have wfΓ := isWAT_wf_local wf.
+  induction sp; try constructor; auto.
+  eapply isWAT_tLetIn_red in wf; auto.
+  specialize (IHsp wf).
+  eapply typing_spine_strengthen; eauto.
+  apply red_cumul. apply red1_red. constructor.
+
+  econstructor; eauto. reflexivity. apply IHsp.
+  eapply isWAT_tProd in wf => //.
+  destruct wf as [wfA wfB].
+  unshelve eapply (@isWAT_subst _ _ wfΣ Γ [vass na A] _ _ [hd]) in wfB => //.
+  constructor; auto.
+  constructor. constructor. now rewrite subst_empty.
+Qed.
+
+Lemma arity_typing_spine {cf:checker_flags} Σ Γ Γ' s inst s' : 
+  wf Σ.1 ->
+  wf_local Σ (Γ ,,, Γ') ->
+  typing_spine Σ Γ (it_mkProd_or_LetIn Γ' (tSort s)) inst (tSort s') ->
+  (#|inst| = context_assumptions Γ') * leq_universe (global_ext_constraints Σ) s s' *
+  ∑ instsubst, spine_subst Σ Γ inst instsubst Γ'.
+Proof.
+  intros wfΣ wfΓ'; revert s inst s'.
+  assert (wf_local Σ Γ). now apply wf_local_app in wfΓ'. move X after wfΓ'.
+  rename X into wfΓ.
+  generalize (le_n #|Γ'|).
+  generalize (#|Γ'|) at 2.
+  induction n in Γ', wfΓ' |- *.
+  - destruct Γ' using rev_ind; try clear IHΓ'; simpl; intros len s inst s' Hsp.
+    + depelim Hsp.
+      ++ intuition auto.
+         now eapply cumul_Sort_inv.
+         exists []. split; try constructor; auto.
+      ++ now eapply cumul_Sort_Prod_inv in c.
+    + rewrite app_length /= in len; elimtype False; lia.
+  - intros len s inst s' Hsp.
+    destruct Γ' using rev_ind; try clear IHΓ'.
+    -- depelim Hsp. 1:intuition auto.
+      --- now eapply cumul_Sort_inv.
+      --- exists []; split; try constructor; auto.
+      --- now eapply cumul_Sort_Prod_inv in c.
+    -- rewrite app_length /= in len.
+      rewrite it_mkProd_or_LetIn_app in Hsp.
+      destruct x as [na [b|] ty]; simpl in *; rewrite /mkProd_or_LetIn /= in Hsp.
+      + rewrite PCUICCtxShape.context_assumptions_app /= Nat.add_0_r.
+        eapply typing_spine_letin_inv in Hsp; auto.
+        rewrite /subst1 subst_it_mkProd_or_LetIn /= in Hsp.
+        specialize (IHn (subst_context [b] 0 l)).
+        forward IHn. {
+          rewrite app_context_assoc in wfΓ'.
+          apply All_local_env_app in wfΓ' as [wfb wfa].
+          depelim wfb. simpl in H; noconf H. simpl in H. noconf H.
+          eapply substitution_wf_local. eauto. 
+          epose proof (cons_let_def Σ Γ [] [] na b ty ltac:(constructor)).
+          rewrite !subst_empty in X. eapply X. auto.
+          eapply All_local_env_app_inv; split.
+          constructor; auto. apply wfa. }
+        forward IHn by rewrite subst_context_length; lia.
+        specialize (IHn s inst s' Hsp). 
+        split. now rewrite context_assumptions_subst in IHn.
+        destruct IHn as [[instlen leq] [instsubst [wfdom wfcodom cs subi]]].
+        exists (instsubst ++ [subst0 [] b]).
+        split; auto.
+        * apply context_subst_app_inv. cbn.
+          rewrite !skipn_0 {1}subst_empty.
+          assert(#|l| <= n) by lia.
+          rewrite context_assumptions_subst in instlen.
+          pose proof (context_subst_length _ _ _ cs). rewrite subst_context_length in H0.
+          rewrite !(firstn_app_left _ 0). lia. simpl. rewrite !app_nil_r.
+          split. now rewrite H0 skipn_all_app.
+          rewrite H0 skipn_all_app. repeat constructor.
+        * apply subslet_app. now rewrite subst_empty.
+          repeat constructor.
+          rewrite app_context_assoc in wfΓ'. simpl in wfΓ'.
+          apply wf_local_app in wfΓ'. depelim wfΓ'; simpl in H; noconf H.
+          now rewrite !subst_empty.
+      + rewrite PCUICCtxShape.context_assumptions_app /=.
+        depelim Hsp. 
+        now eapply cumul_Prod_Sort_inv in c.
+        eapply cumul_Prod_inv in c as [conva cumulB].
+        eapply (substitution_cumul0 _ _ _ _ _ _ hd) in cumulB; auto.
+        rewrite /subst1 subst_it_mkProd_or_LetIn /= in cumulB.
+        specialize (IHn (subst_context [hd] 0 l)).
+        forward IHn. {
+          rewrite app_context_assoc in wfΓ'.
+          apply All_local_env_app in wfΓ' as [wfb wfa]; eauto.
+          depelim wfb. simpl in H; noconf H.
+          eapply substitution_wf_local. auto. 
+          constructor. constructor. rewrite subst_empty.
+          eapply type_Cumul. eapply t.
+          right; eapply l0.
+          eapply conv_cumul; auto. now symmetry. 
+          eapply All_local_env_app_inv; eauto; split.
+          constructor; eauto. eapply isWAT_tProd in i; intuition eauto.
+          simpl in H; noconf H.
+        }
+        forward IHn by rewrite subst_context_length; lia.
+        specialize (IHn s tl s'). 
+        rewrite context_assumptions_subst in IHn.
+        eapply typing_spine_strengthen in Hsp.
+        3:eapply cumulB. all:eauto.
+        simpl. specialize (IHn Hsp).
+        destruct IHn as [[instlen leq] [instsubst [wfdom wfcodom cs subi]]].
+        intuition auto. lia.
+        exists (instsubst ++ [hd]).
+        split; auto.
+        * apply context_subst_app_inv. cbn.
+          rewrite !skipn_S skipn_0.
+          assert(#|l| <= n) by lia.
+          pose proof (context_subst_length _ _ _ cs). rewrite subst_context_length in H0.
+          rewrite !(firstn_app_left _ 0). lia. simpl. rewrite !app_nil_r.
+          split. now rewrite H0 skipn_all_app.
+          rewrite H0 skipn_all_app. apply (context_subst_ass _ []). constructor.
+        * apply subslet_app => //.
+          repeat constructor.
+          rewrite app_context_assoc in wfΓ'. simpl in wfΓ'.
+          apply wf_local_app in wfΓ'. depelim wfΓ'; simpl in H; noconf H.
+          rewrite !subst_empty. red in l0.
+          eapply type_Cumul; eauto. eapply conv_cumul. now symmetry.
+Qed.
+
+Lemma typing_spine_it_mkProd_or_LetIn_gen {cf:checker_flags} Σ Γ Δ Δ' T args s s' args' T' : 
+  wf Σ.1 ->
+  make_context_subst (List.rev Δ) args s' = Some s -> 
+  typing_spine Σ Γ (subst0 s T) args' T' ->
+  #|args| = context_assumptions Δ ->
+  subslet Σ Γ s (Δ' ,,, Δ) ->
+  isWfArity_or_Type Σ Γ (it_mkProd_or_LetIn Δ' (it_mkProd_or_LetIn Δ T)) ->
+  typing_spine Σ Γ (subst0 s' (it_mkProd_or_LetIn Δ T)) (args ++ args') T'.
+Proof.
+  intros wfΣ.
+  generalize (le_n #|Δ|).
+  generalize (#|Δ|) at 2.
+  induction n in Δ, Δ', args, s, s', T |- *.
+  - destruct Δ using rev_ind.
+    + intros le Hsub Hsp.
+      destruct args; simpl; try discriminate.
+      simpl in Hsub. now depelim Hsub.
+    + rewrite app_length /=; intros; elimtype False; lia.
+  - destruct Δ using rev_ind.
+    1:intros le Hsub Hsp; destruct args; simpl; try discriminate;
+    simpl in Hsub; now depelim Hsub.
+  clear IHΔ.
+  rewrite app_length /=; intros Hlen Hsub Hsp Hargs.
+  rewrite context_assumptions_app in Hargs.
+  destruct x as [na [b|] ty]; simpl in *.
+  * rewrite it_mkProd_or_LetIn_app /= /mkProd_or_LetIn /=.
+    rewrite Nat.add_0_r in Hargs.
+    rewrite rev_app_distr in Hsub. simpl in Hsub.
+    intros subs. rewrite app_context_assoc in subs.
+    specialize (IHn Δ _ T args s _ ltac:(lia) Hsub Hsp Hargs subs).
+    intros Har. forward IHn.
+    rewrite it_mkProd_or_LetIn_app.
+    now simpl.
+    eapply typing_spine_letin; auto.
+    rewrite /subst1.
+    now rewrite -subst_app_simpl.
+  * rewrite it_mkProd_or_LetIn_app /= /mkProd_or_LetIn /=.
+    rewrite rev_app_distr in Hsub. 
+    simpl in Hsub. destruct args; try discriminate.
+    simpl in Hargs. rewrite Nat.add_1_r in Hargs. noconf Hargs. simpl in H; noconf H.
+    intros subs. rewrite app_context_assoc in subs.    
+    specialize (IHn Δ _ T args s _ ltac:(lia) Hsub Hsp H subs).
+    intros Har.
+    forward IHn. now rewrite it_mkProd_or_LetIn_app.
+    eapply subslet_app_inv in subs as [subsl subsr].
+    depelim subsl; simpl in H1; noconf H1.
+    have Hskip := make_context_subst_skipn Hsub. 
+    rewrite List.rev_length in Hskip. rewrite Hskip in H0; noconf H0.
+    simpl; eapply typing_spine_prod; auto; first
+    now rewrite /subst1 -subst_app_simpl.
+    eapply isWAT_it_mkProd_or_LetIn_app in Har; eauto.
+Qed.
+
+Lemma typing_spine_it_mkProd_or_LetIn {cf:checker_flags} Σ Γ Δ T args s args' T' : 
+  wf Σ.1 ->
+  make_context_subst (List.rev Δ) args [] = Some s -> 
+  typing_spine Σ Γ (subst0 s T) args' T' ->
+  #|args| = context_assumptions Δ ->
+  subslet Σ Γ s Δ ->
+  isWfArity_or_Type Σ Γ (it_mkProd_or_LetIn Δ T) ->
+  typing_spine Σ Γ (it_mkProd_or_LetIn Δ T) (args ++ args') T'.
+Proof.
+  intros. 
+  pose proof (typing_spine_it_mkProd_or_LetIn_gen Σ Γ Δ [] T args s [] args' T'); auto.
+  now rewrite subst_empty app_context_nil_l in X3.
+Qed.
+
+Lemma typing_spine_it_mkProd_or_LetIn' {cf:checker_flags} Σ Γ Δ T args s args' T' : 
+  wf Σ.1 ->
+  spine_subst Σ Γ args s Δ ->
+  typing_spine Σ Γ (subst0 s T) args' T' ->
+  isWfArity_or_Type Σ Γ (it_mkProd_or_LetIn Δ T) ->
+  typing_spine Σ Γ (it_mkProd_or_LetIn Δ T) (args ++ args') T'.
+Proof.
+  intros. destruct X0.
+  eapply typing_spine_it_mkProd_or_LetIn; eauto.
+  eapply make_context_subst_spec_inv. now rewrite List.rev_involutive.
+  now pose proof (context_subst_length2 inst_ctx_subst0).
+Qed.
+
+Lemma typing_spine_it_mkProd_or_LetIn_close {cf:checker_flags} Σ Γ Δ T args s : 
+  wf Σ.1 ->
+  make_context_subst (List.rev Δ) args [] = Some s -> 
+  #|args| = context_assumptions Δ ->
+  subslet Σ Γ s Δ ->
+  isWfArity_or_Type Σ Γ (it_mkProd_or_LetIn Δ T) ->
+  typing_spine Σ Γ (it_mkProd_or_LetIn Δ T) args (subst0 s T).
+Proof.
+  intros. 
+  pose proof (typing_spine_it_mkProd_or_LetIn_gen Σ Γ Δ [] T args s [] []); auto.
+  rewrite app_nil_r subst_empty in X2. apply X2; eauto.
+  constructor. 2:eauto.
+  eapply isWAT_it_mkProd_or_LetIn_app; eauto with pcuic. pcuic.
+  now rewrite app_context_nil_l.
+Qed.
+
+Lemma typing_spine_it_mkProd_or_LetIn_close_eq {cf:checker_flags} Σ Γ Δ T args s T' : 
+  wf Σ.1 ->
+  make_context_subst (List.rev Δ) args [] = Some s -> 
+  #|args| = context_assumptions Δ ->
+  subslet Σ Γ s Δ ->
+  isWfArity_or_Type Σ Γ (it_mkProd_or_LetIn Δ T) ->
+  T' = (subst0 s T) ->
+  typing_spine Σ Γ (it_mkProd_or_LetIn Δ T) args T'.
+Proof.
+  intros; subst; now apply typing_spine_it_mkProd_or_LetIn_close.
+Qed. 
+
+Lemma typing_spine_it_mkProd_or_LetIn_close' {cf:checker_flags} Σ Γ Δ T args s T' : 
+  wf Σ.1 ->
+  spine_subst Σ Γ args s Δ ->
+  isWfArity_or_Type Σ Γ (it_mkProd_or_LetIn Δ T) ->
+  T' = (subst0 s T) ->
+  typing_spine Σ Γ (it_mkProd_or_LetIn Δ T) args T'.
+Proof.
+  intros wfΣ [].
+  intros; eapply typing_spine_it_mkProd_or_LetIn_close_eq; eauto.
+  eapply make_context_subst_spec_inv.
+  now rewrite List.rev_involutive.
+  now eapply context_subst_length2 in inst_ctx_subst0.
+Qed. 
+
+
+Lemma context_subst_subst Δ inst0 s Γ inst s'  :
+  context_subst Δ inst0 s ->
+  context_subst (subst_context s 0 Γ) inst s' ->
+  context_subst (Δ ,,, Γ) (inst0 ++ inst) (s' ++ s).
+Proof.
+induction Γ in inst, s' |- *.
++ intros HΔ Hi. depelim Hi.
+  now rewrite app_nil_r.
++ intros H' Hsub. 
+  rewrite subst_context_snoc0 in Hsub.
+  destruct a as [na [b|] ty];
+  depelim Hsub; simpl in H; noconf H.
+  - specialize (IHΓ _ _ H' Hsub).
+    assert(#|Γ| = #|s0|) as ->.
+    { apply context_subst_length in Hsub.
+      now rewrite subst_context_length in Hsub. }
+    rewrite -(subst_app_simpl s0 s 0 b).
+    simpl. now constructor.
+  - specialize (IHΓ _ _ H' Hsub).
+    assert(#|Γ| = #|s0|).
+    { apply context_subst_length in Hsub.
+      now rewrite subst_context_length in Hsub. }
+    rewrite app_assoc /=. now constructor.
+Qed.
+
+Lemma spine_subst_conv {cf:checker_flags} Σ Γ inst insts Δ inst' insts' Δ' :
+  wf Σ.1 ->
+  spine_subst Σ Γ inst insts Δ ->
+  spine_subst Σ Γ inst' insts' Δ' ->
+  context_relation (fun Δ Δ' => conv_decls Σ (Γ ,,, Δ) (Γ ,,, Δ')) Δ Δ' ->
+  All2 (conv Σ Γ) inst inst' -> All2 (conv Σ Γ) insts insts'.
+Proof.
+move=> wfΣ [_ wf cs sl] [_ _ cs' sl'] cv.
+move: inst insts cs wf sl inst' insts' cs' sl'.
+induction cv; intros; depelim cs ; depelim cs';
+  try (simpl in H; noconf H); try (simpl in H0; noconf H0).
+- constructor; auto.    
+- eapply All2_app_inv in X as [[l1 l2] [[? ?] ?]].
+  depelim a2. depelim a2. apply app_inj_tail in e as [? ?]; subst.
+  depelim sl; depelim sl'; simpl in H; noconf H; simpl in H0; noconf H0;
+    try (simpl in H1; noconf H1).
+  depelim wf; simpl in H; noconf H.
+  specialize (IHcv _ _ cs wf sl _ _ cs' sl' a1).
+  constructor; auto.
+- depelim sl; depelim sl'; simpl in H; noconf H; simpl in H0; noconf H0;
+    try (simpl in H1; noconf H1); try (simpl in H2; noconf H2).
+  depelim wf; simpl in H; noconf H.
+  specialize (IHcv _ _ cs wf sl _ _ cs' sl' X).
+  constructor; auto.
+  eapply (subst_conv _ _ _ []); eauto.
+  depelim p; pcuic.
+Qed.
+
+Lemma spine_subst_subst {cf:checker_flags} Σ Γ Γ0 Γ' i s Δ sub : 
+  wf Σ.1 ->
+  spine_subst Σ (Γ ,,, Γ0 ,,, Γ') i s Δ ->
+  subslet Σ Γ sub Γ0 ->
+  spine_subst Σ (Γ ,,, subst_context sub 0 Γ') (map (subst sub #|Γ'|) i) (map (subst sub #|Γ'|) s)
+   (subst_context sub #|Γ'| Δ).
+Proof.
+  move=> wfΣ [wfl wfΔ cs subl] subs.
+  split.
+  eapply substitution_wf_local; eauto.
+  pose proof (subst_context_app sub 0 Γ' Δ). rewrite Nat.add_0_r in H. rewrite -app_context_assoc -H.
+  clear H.
+  eapply substitution_wf_local; eauto. now rewrite app_context_assoc.
+  clear subl wfl wfΔ.
+  induction cs in Γ, Γ0, Γ', subs |- *; rewrite ?subst_context_snoc ?map_app; simpl; try constructor.
+  eapply IHcs; eauto.
+  specialize (IHcs _ _ Γ' subs).
+  epose proof (context_subst_def _ _ _ na (subst sub (#|Γ1| + #|Γ'|) b) (subst sub (#|Γ1| + #|Γ'|) t) IHcs).
+  rewrite /subst_decl /map_decl /=.
+  rewrite distr_subst. 
+  now rewrite (context_subst_length _ _ _ cs) in X |- *.
+  clear cs wfΔ.
+  induction subl; rewrite ?subst_context_snoc ?map_app; simpl; try constructor; auto.
+  - eapply substitution in t0; eauto. simpl.
+    rewrite -(subslet_length subl).
+    now rewrite -distr_subst.
+  - eapply substitution in t0; eauto. simpl.
+    rewrite -(subslet_length subl).
+    rewrite !distr_subst in t0.
+    epose proof (cons_let_def _  _ _ _ _  _ _ IHsubl t0).
+    now rewrite - !distr_subst in X.
+Qed.
+
+Lemma weaken_subslet {cf:checker_flags} Σ s Δ Γ Γ' :
+  wf Σ.1 ->
+  wf_local Σ Γ -> wf_local Σ Γ' ->
+  subslet Σ Γ' s Δ -> subslet Σ (Γ ,,, Γ') s Δ.
+Proof.
+  intros wfΣ wfΔ wfΓ'.
+  induction 1; constructor; auto.
+  + eapply (weaken_ctx Γ); eauto.
+  + eapply (weaken_ctx Γ); eauto.
+Qed.
+
+Lemma spine_subst_weaken {cf:checker_flags} Σ Γ i s Δ Γ' : 
+  wf Σ.1 ->
+  wf_local Σ Γ' ->
+  spine_subst Σ Γ i s Δ ->
+  spine_subst Σ (Γ' ,,, Γ) i s Δ.
+Proof.
+  move=> wfΣ wfl [cs subl].
+  split; auto.
+  eapply weaken_wf_local => //.
+  rewrite -app_context_assoc. eapply weaken_wf_local => //.
+  eapply weaken_subslet; eauto.
+Qed.
+
+
+
+Lemma spine_subst_app_inv {cf:checker_flags} Σ Γ Δ Δ' inst inst' insts :
+  wf Σ.1 -> 
+  #|inst| = context_assumptions Δ ->
+  spine_subst Σ Γ (inst ++ inst') insts (Δ ,,, Δ') ->
+  spine_subst Σ Γ inst (skipn #|Δ'| insts) Δ *
+  spine_subst Σ Γ inst' (firstn #|Δ'| insts) (subst_context (skipn #|Δ'| insts) 0 Δ').
+Proof.
+  intros wfΣ len sp.
+  destruct sp as [wfdom wfcodom cs subs].
+  eapply context_subst_app in cs as [csl csr].
+  rewrite skipn_all_app_eq in csl => //.
+  rewrite (firstn_app_left _ 0) in csr => //. lia.
+  rewrite firstn_0 in csr => //. rewrite app_nil_r in csr.
+  eapply subslet_app_inv in subs as [sl sr].
+  split; split; auto. rewrite app_context_assoc in wfcodom.
+  now eapply All_local_env_app in wfcodom as [? ?].
+  eapply substitution_wf_local; eauto.
+  now rewrite app_context_assoc in wfcodom.
+Qed.
+
+Lemma spine_subst_inst {cf:checker_flags} Σ ext u Γ i s Δ  :
+  wf Σ.1 ->
+  wf_global_ext Σ.1 ext ->
+  spine_subst (Σ.1, ext) Γ i s Δ ->
+  consistent_instance_ext Σ ext u ->
+  spine_subst Σ (subst_instance_context u Γ)
+    (map (subst_instance_constr u) i)
+    (map (subst_instance_constr u) s)
+    (subst_instance_context u Δ).
+Proof.
+  intros wfΣ wfext [wfdom wfcodom cs subsl] cu.
+  split.
+  eapply wf_local_subst_instance; eauto.
+  rewrite -subst_instance_context_app.
+  eapply wf_local_subst_instance; eauto.
+  clear -cs cu wfext wfΣ.
+  induction cs; simpl; rewrite ?map_app; try constructor; auto.
+  simpl.
+  rewrite -subst_subst_instance_constr.
+  constructor; auto.
+
+  clear -subsl cu wfΣ wfext.
+  induction subsl; simpl; rewrite -?subst_subst_instance_constr; constructor; auto.
+  * destruct Σ as [Σ univs].
+    rewrite subst_subst_instance_constr.
+    eapply (typing_subst_instance'' Σ); simpl; auto.
+    apply wfext. simpl in wfext. apply t0. 
+    apply wfext. auto.
+  * rewrite !subst_subst_instance_constr. simpl.
+    destruct Σ as [Σ univs].
+    eapply (typing_subst_instance'' Σ); simpl; auto.
+    apply wfext. simpl in wfext. apply t0. 
+    apply wfext. auto.
+Qed.
+
+Lemma subslet_lift {cf:checker_flags} Σ (Γ Δ : context) s Δ' :
+  wf Σ.1 -> wf_local Σ (Γ ,,, Δ) ->
+  subslet Σ Γ s Δ' ->
+  subslet Σ (Γ ,,, Δ) (map (lift0 #|Δ|) s) (lift_context #|Δ| 0 Δ').
+Proof.
+  move=> wfΣ wfl.
+  induction 1; rewrite ?lift_context_snoc /=; try constructor; auto.
+  simpl.
+  rewrite -(subslet_length X).
+  rewrite -distr_lift_subst. apply weakening; eauto.
+
+  rewrite -(subslet_length X).
+  rewrite distr_lift_subst. constructor; auto.
+  rewrite - !distr_lift_subst. apply weakening; eauto.
+Qed.
+
+Lemma spine_subst_weakening {cf:checker_flags} Σ Γ i s Δ Γ' : 
+  wf Σ.1 ->
+  wf_local Σ (Γ ,,, Γ') ->
+  spine_subst Σ Γ i s Δ ->
+  spine_subst Σ (Γ ,,, Γ') (map (lift0 #|Γ'|) i) (map (lift0 #|Γ'|) s) (lift_context #|Γ'| 0 Δ).
+Proof.
+  move=> wfΣ wfl [cs subl].
+  split; auto.
+  eapply weakening_wf_local; eauto.
+  now apply context_subst_lift.
+  now apply subslet_lift.
+Qed.
